examples/lowparse/LowParse.Int.fst
@@ -14,18 +14,56 @@ let parse_u8: total_constant_size_parser 1 U8.t =
   make_total_constant_size_parser 1 U8.t (fun b -> Seq.index b 0)
 
 noextract
+let decode_u16
+  (b: bytes32 { Seq.length b == 2 } )
+: Tot U16.t
+= E.lemma_be_to_n_is_bounded b;
+  U16.uint_to_t (E.be_to_n b)
+
+noextract
 let parse_u16: total_constant_size_parser 2 U16.t =
-  make_total_constant_size_parser 2 U16.t (fun b' ->
-          E.lemma_be_to_n_is_bounded b';
-          U16.uint_to_t (E.be_to_n b')
-  )
+  make_total_constant_size_parser 2 U16.t decode_u16
+
+noextract
+let decode_u32
+  (b: bytes32 { Seq.length b == 4 } )
+: Tot U32.t
+= E.lemma_be_to_n_is_bounded b;
+  U32.uint_to_t (E.be_to_n b)
 
 noextract
 let parse_u32: total_constant_size_parser 4 U32.t =
-  make_total_constant_size_parser 4 U32.t (fun b' ->
-          E.lemma_be_to_n_is_bounded b';
-          U32.uint_to_t (E.be_to_n b')
-  )
+  make_total_constant_size_parser 4 U32.t decode_u32
+
+let parse_u8_injective () : Lemma (injective parse_u8) =
+  assert (forall (b1: bytes32 { Seq.length b1 == 1 }) (b2: bytes32 { Seq.length b2 == 1 }) .
+    Seq.index b1 0 == Seq.index b2 0 ==> Seq.equal b1 b2
+  );
+  make_total_constant_size_parser_injective 1 U8.t (fun b -> Seq.index b 0)
+
+let parse_u16_injective () : Lemma (injective parse_u16) =
+  assert (forall (b1: bytes32 { Seq.length b1 == 2 }) (b2: bytes32 { Seq.length b2 == 2 }) .
+    decode_u16 b1 == decode_u16 b2 ==> Seq.equal b1 b2
+  );
+  make_total_constant_size_parser_injective 2 U16.t decode_u16
+
+#set-options "--z3rlimit 32 --max_fuel 8 --max_ifuel 8"
+
+let parse_u32_injective () : Lemma (injective parse_u32) =
+  assert (forall (b1: bytes32 { Seq.length b1 == 4 }) (b2: bytes32 { Seq.length b2 == 4 }) .
+    decode_u32 b1 == decode_u32 b2 ==> (
+      Seq.index b1 0 == Seq.index b2 0 /\
+      Seq.index b1 1 == Seq.index b2 1 /\
+      Seq.index b1 2 == Seq.index b2 2 /\
+      Seq.index b1 3 == Seq.index b2 3
+  ));
+  assert (forall (b1: bytes32 { Seq.length b1 == 4 }) (b2: bytes32 { Seq.length b2 == 4 }) .
+    decode_u32 b1 == decode_u32 b2 ==> (
+      Seq.equal b1 b2
+  ));
+  make_total_constant_size_parser_injective 4 U32.t decode_u32
+
+#reset-options
 
 [@"substitute"]
 inline_for_extraction
@@ -83,5 +121,3 @@ let parse_u32_st_nochk :
 inline_for_extraction
 let parse_u32_st : parser_st (parse_u32) =
   parse_total_constant_size 4ul parse_u32_st_nochk
-
-let parse_byte: total_constant_size_parser 1 byte = parse_u8
